bidirectional/theories/BDMinimalToPCUIC.v
@@ -1,0 +1,491 @@
+From Coq Require Import Bool List Arith Lia.
+From MetaCoq.Template Require Import config utils monad_utils.
+From MetaCoq.PCUIC Require Import PCUICAst PCUICLiftSubst PCUICTyping PCUICInversion PCUICInductiveInversion.
+From MetaCoq.PCUIC Require Import PCUICWeakening PCUICClosed PCUICSubstitution PCUICPrincipality PCUICValidity PCUICCumulativity.
+From MetaCoq.PCUIC Require Import PCUICWfUniverses PCUICSR.
+From MetaCoq.Bidirectional Require Import BDEnvironmentTyping BDMinimalTyping.
+
+Require Import ssreflect.
+From Equations Require Import Equations.
+Require Import Equations.Prop.DepElim.
+
+Module PT := PCUIC.PCUICTyping.
+Module MT := Bidirectional.BDMinimalTyping.
+
+Section BDMinimalToPCUICTyping.
+
+  Let Pcheck `{checker_flags} Σ Γ t T :=
+    PT.wf_local Σ Γ -> PT.isType Σ Γ T -> Σ ;;; Γ |- t : T.
+
+  Let Pinfer `{checker_flags} Σ Γ t T :=
+    PT.wf_local Σ Γ -> Σ ;;; Γ |- t : T.
+
+  Let Psort `{checker_flags} Σ Γ t u :=
+    PT.wf_local Σ Γ -> Σ ;;; Γ |- t : (tSort u).
+
+  Let Pprod `{checker_flags} Σ Γ t na A B :=
+    PT.wf_local Σ Γ -> Σ ;;; Γ |- t : tProd na A B.
+
+  Let Pind `{checker_flags} Σ Γ ind t u args :=
+    PT.wf_local Σ Γ -> Σ ;;; Γ |- t : mkApps (tInd ind u) args.
+
+  Let PΓ `{checker_flags} Σ Γ (wfΓ : wf_local Σ Γ) :=
+    PT.wf_local Σ Γ.
+
+  Lemma wf_arities_context' {cf:checker_flags}:
+    forall (Σ : global_env_ext) (mdecl : mutual_inductive_body),
+      PT.wf Σ ->
+      All (fun idecl => PT.on_type (PT.lift_typing typing) Σ [] (ind_type idecl)) (ind_bodies mdecl) ->
+      PT.wf_local Σ (arities_context (ind_bodies mdecl)).
+  Proof.
+    intros Σ mdecl wfΣ Hdecl.
+    unfold arities_context.
+    revert Hdecl.
+    induction (ind_bodies mdecl) using rev_ind. 1: constructor.
+    intros Ha.
+    rewrite rev_map_app.
+    simpl.    
+    apply All_app in Ha as [Hl Hx].
+    inv Hx. clear X0.
+    destruct X as [s Hs].
+    specialize (IHl Hl).
+    econstructor; eauto.
+    fold (arities_context l) in *.
+    unshelve epose proof (weakening Σ [] (arities_context l) _ _ wfΣ _ Hs).
+    1: now rewrite app_context_nil_l.
+    simpl in X.
+    simpl.
+    eapply (env_prop_typing _ _ typecheck_closed) in Hs; eauto.
+    rewrite -> andb_and in Hs. destruct Hs as [Hs Ht].
+    simpl in Hs. apply (lift_closed #|arities_context l|) in Hs.
+    rewrite -> Hs, app_context_nil_l in X. simpl. exists s.
+    apply X.
+  Qed.
+
+Lemma bd_wf_local `{checker_flags} Σ Γ (all: wf_local Σ Γ) :
+  MT.All_local_env_over_sorting checking infering_sort 
+    (fun Σ Γ _ t T _ => Pcheck Σ Γ t T)
+    (fun Σ Γ _ t u _ => Psort Σ Γ t u) 
+    Σ Γ all ->
+  PT.wf_local Σ Γ.
+Proof.
+  intros allo ; induction allo.
+  all: constructor.
+  1,3: assumption.
+  all: red.
+  - simpl in t0. eexists.
+    auto.
+  - destruct t0. eexists.
+    auto.
+  - destruct t0.
+    apply p0 ; auto.
+    eexists. red. auto.
+Qed.
+
+Lemma type_local_ctx_impl `{checker_flags} Σ Γ Δ u (wfΓ : PT.wf_local Σ Γ):
+  type_local_ctx Pcheck Psort Σ Γ Δ u -> PT.type_local_ctx (lift_typing typing) Σ Γ Δ u.
+Proof.
+  intros HΔ.
+  induction Δ as [|[? []]].
+  1: auto.
+  all: simpl.
+  1: destruct HΔ as ((?&[])&?).
+  2: destruct HΔ.
+  all: have wfΓΔ : PT.wf_local Σ (Γ ,,, Δ) by eapply PCUICContexts.type_local_ctx_wf_local ; eauto.
+  all: repeat split ; auto.
+  ++ eexists. eauto.
+  ++ apply l.
+     2: eexists ; eapply p.
+     all: eauto.
+Qed.
+
+Lemma bd_wf `{checker_flags} Σ : Forall_decls_sorting Pcheck Psort Σ -> PT.wf Σ.
+Proof.
+  intros wfΣ. induction wfΣ.
+  all: constructor.
+  - assumption.
+  - assumption.
+  - constructor ; intuition.
+  - destruct d as [[? [] ?]|].
+    + inversion o0 as [[u Hty] Hb].
+      apply Hb.
+      1: constructor.
+      exists u.
+      simpl.
+      eapply Hty.
+      constructor.
+    + inversion o0. eexists.
+      eauto.
+    + destruct o0.
+      have wf_arities : PT.wf_local (Σ,udecl) (arities_context (ind_bodies m)).
+      { apply wf_arities_context'.
+        1: assumption.
+        induction onInductives.
+        all: constructor ; auto.
+        destruct p.
+        destruct onArity as [? onArity].
+        eexists.
+        eapply onArity.
+        constructor. }
+      have wf_params : PT.wf_local (Σ,udecl) (ind_params m).
+      { clear - onParams.
+        induction onParams.
+        all: constructor.
+        all: auto.
+        1: by destruct t0 ; eexists ; eauto.
+        1: by destruct t0 as ((? & ?) & ?) ; eexists ; eauto.
+        destruct t0 as ((? & ?)&c).
+        apply c.
+        1: auto.
+        eexists. red. eauto. }
+
+      constructor ; auto.
+      
+      remember (ind_bodies m) as l in onInductives |- *.
+      clear - IHwfΣ onInductives wf_arities wf_params.
+      induction onInductives.
+      all: constructor ; auto.
+      destruct p.
+      unshelve econstructor.
+      * exact ind_indices.
+      * exact ind_sort.
+      * eapply map.
+        2: exact ind_cshapes.
+        intros [].
+        constructor ; auto.
+      * assumption.
+      * destruct onArity as [? onArity].
+        eexists.
+        eapply onArity.
+        constructor.
+      * apply All2_map_right.
+        eapply All2_impl.
+        1: exact onConstructors.
+        intros [[] ?] [] [] ; simpl in *.
+
+        have wf_args : PT.wf_local (Σ,udecl) (arities_context (ind_bodies m),,,(ind_params m),,, cshape_args).
+        { eapply PCUICContexts.type_local_ctx_wf_local.
+          1: by apply weaken_wf_local.
+          eapply type_local_ctx_impl ; eauto.
+          by apply weaken_wf_local. }
+
+        constructor ; auto ; simpl in *.
+
+        --destruct on_ctype as [? on_ctype].
+          eexists.
+          apply on_ctype.
+          1: eassumption.
+        --apply type_local_ctx_impl ; eauto.
+          apply weaken_wf_local.
+          all: auto.
+
+        --match goal with |- PT.ctx_inst _ _ ?ctx _ _ => remember ctx as Γ' end.
+          clear -on_cindices wf_args.
+          induction on_cindices.
+          all: constructor.
+          2-3: assumption.
+          apply l0 ; auto.
+          destruct l.
+          eexists. red. eauto.
+
+        --clear - on_ctype_positive.
+          cbn in on_ctype_positive |- *.
+          induction on_ctype_positive.
+          all: constructor ; auto.
+          clear - p. induction p.
+          ++constructor ; assumption.
+          ++econstructor 2 ; eauto.
+          ++constructor 3 ; auto.
+          ++constructor 4 ; auto.
+        --clear - on_ctype_variance.
+          intros v e.
+          specialize (on_ctype_variance v e).
+          unfold cstr_respects_variance in on_ctype_variance.
+          unfold PT.cstr_respects_variance.
+          destruct (variance_universes (PCUICEnvironment.ind_universes m)) ; simpl in * ; auto.
+          destruct p as [[]]. intuition.
+          induction a.
+          all: constructor ; auto.
+
+        
+      * intros projs ; specialize (onProjections projs).
+        clear - onProjections.
+        induction ind_cshapes.
+        1: auto.
+        simpl in *.
+        destruct ind_cshapes.
+        { destruct a. simpl in *.
+          destruct onProjections. constructor ; intuition. }
+        assumption.
+
+      * clear -ind_sorts wf_params.
+        cbn in *.
+        red in ind_sorts |- *.
+        destruct (universe_family ind_sort).
+        --induction ind_cshapes ; auto.
+        --induction ind_cshapes ; auto.
+          simpl in *.
+          destruct ind_cshapes ; auto.
+          simpl in *.
+          destruct a ; auto.
+        --destruct ind_sorts. split.
+          { apply Forall_map.
+            eapply Forall_impl. 1: eassumption.
+            intros [] ? ; assumption. }
+          destruct indices_matter ; auto.
+          apply type_local_ctx_impl.
+          all: auto.
+        --destruct ind_sorts. split.
+          { apply Forall_map.
+            eapply Forall_impl. 1: eassumption.
+            intros [] ? ; assumption. }
+          destruct indices_matter ; auto.
+          apply type_local_ctx_impl.
+          all: auto.
+
+      *  clear -onIndices.
+        intros v e. specialize (onIndices v e).
+        unfold ind_respects_variance in onIndices.
+        unfold PT.ind_respects_variance.
+        destruct (PCUICEnvironment.ind_universes m) ; simpl in * ; auto.
+        destruct cst.
+        replace (PT.level_var_instance 0 l) with (level_var_instance 0 l).
+        2:{ by induction l ; auto. }
+        match goal with |- context [PT.lift_instance ?len ?list] =>
+        replace (PT.lift_instance len list) with (lift_instance len list) end.
+        2:{ apply map_ext. intros []. all: reflexivity. }
+        induction onIndices.
+        all: constructor ; auto.
+Qed.
+  
+Theorem bidirectional_to_PCUIC `{cf : checker_flags} : env_prop Pcheck Pinfer Psort Pprod Pind (@PΓ).
+Proof.
+  apply MT.typing_ind_env.
+
+  { intros. eapply bd_wf_local. eassumption. }
+
+  1-14: intros ; red ; econstructor ; eauto.
+
+  - apply X2.
+    constructor. 1: by auto.
+    eexists. eauto.
+
+  - apply X2.
+    constructor. 1: by auto.
+    eexists. eauto.
+  
+  - apply X2 ; auto.
+    eexists.
+    red. eauto.
+  
+  - apply X4.
+    constructor ; auto.
+    + eexists. eauto.
+    + apply X2 ; auto. eexists. red. eauto.
+  
+  - apply X2 ; auto.
+    specialize (X0 X3).
+    apply validity in X0.
+    2: by apply bd_wf.
+    destruct X0 as [? X0].
+    apply inversion_Prod in X0.
+    2: by apply bd_wf.
+    destruct X0 as (? & ? & ? & _).
+    eexists. eassumption.
+
+  - apply X3 ; auto.
+    suff [] : @isWfArity cf Σ Γ pty by done.
+    eapply WfArity_build_case_predicate_type.
+    + by apply bd_wf.
+    + case isdecl ; split ; eauto.
+    + eapply validity.
+      1: by apply bd_wf.
+      by auto.
+    + eassumption.
+    + unfold params in * ; rewrite <- H0 in * ; eassumption.
+
+  - clear H4.
+    induction X4.
+    all: constructor ; auto.
+    destruct r as (? & ? & ? & ? & ?).
+    repeat split ; auto.
+    apply p1 ; auto.
+    all: eexists.
+    all: apply p0.
+    all: by auto.
+
+  - clear H H0 H1 X0.
+    induction X.
+    all: constructor ; auto.
+    destruct p as (? & ? & ?).
+    eexists.
+    apply p.
+    auto.
+
+  - have Htypes : All (fun d => PT.isType Σ Γ (dtype d)) mfix.
+    { clear H H0 H1 X0.
+      induction X.
+      all: constructor ; auto.
+      destruct p as (? & ? & ?).
+      eexists.
+      apply p.
+      auto.
+    }
+    have wfΓ' : PT.wf_local Σ (Γ,,,fix_context mfix).
+    { apply All_mfix_wf ; auto.
+      by apply bd_wf.
+    }
+    remember (fix_context mfix) as Γ'.
+    clear H H0 H1 HeqΓ'.
+    induction X0.
+    all: constructor ; auto.
+    2:{ inversion_clear X. apply IHX0 ; auto. inversion_clear Htypes. auto. }
+    destruct p as (? & ? & ?).
+    split ; auto.
+    apply p ; auto.
+    inversion_clear Htypes as [| ? ? [u]].
+    exists u.
+    change (tSort u) with (lift0 #|Γ'| (tSort u)).
+    apply weakening.
+    all: auto.
+    by apply bd_wf.
+
+    - clear H H0 H1 X0.
+    induction X.
+    all: constructor ; auto.
+    destruct p as (? & ? & ?).
+    eexists.
+    apply p.
+    auto.
+
+  - have Htypes : All (fun d => PT.isType Σ Γ (dtype d)) mfix.
+    { clear H H0 H1 X0.
+      induction X.
+      all: constructor ; auto.
+      destruct p as (? & ? & ?).
+      eexists.
+      apply p.
+      auto.
+    }
+    have wfΓ' : PT.wf_local Σ (Γ,,,fix_context mfix).
+    { apply All_mfix_wf ; auto.
+      by apply bd_wf.
+    }
+    remember (fix_context mfix) as Γ'.
+    clear H H0 H1 HeqΓ'.
+    induction X0.
+    all: constructor ; auto.
+    2:{ inversion_clear X. apply IHX0 ; auto. inversion_clear Htypes. auto. }
+    destruct p.
+    apply p ; auto.
+    inversion_clear Htypes as [| ? ? [u]].
+    exists u.
+    change (tSort u) with (lift0 #|Γ'| (tSort u)).
+    apply weakening.
+    all: auto.
+    by apply bd_wf.
+
+  - constructor ; auto.
+    suff wfu : (wf_universes Σ (tSort u)) by apply (reflect_bP (wf_universe_reflect _ u)).
+    eapply isType_wf_universes.
+    1: by apply bd_wf.
+    eapply isType_red.
+    1: by apply bd_wf.
+    1: eauto.
+    eapply validity_term.
+    1: by apply bd_wf.
+    auto.
+
+  - apply red_cumul.
+    assumption.
+  
+  - intros. red. intro.
+    have [] : (PT.isType Σ Γ (tProd na A B)).
+    { eapply isType_red.
+      1: by apply bd_wf.
+      1: eauto.
+      eapply validity_term.
+      1: by apply bd_wf.
+      auto.
+    }
+    econstructor.
+    + by auto.
+    + by eassumption.
+    + by apply red_cumul. 
+  
+  - intros. red. intro.
+    have [] : (PT.isType Σ Γ (mkApps (tInd ind ui) args)).
+    { eapply isType_red.
+      1: by apply bd_wf.
+      1: eauto.
+      eapply validity_term.
+      1: by apply bd_wf.
+      auto.
+    }
+    econstructor.
+    + by auto.
+    + by eassumption.
+    + by apply red_cumul. 
+
+  - intros. red. intros ? [].
+    econstructor.
+    all:by eauto.
+
+Qed.
+
+End BDMinimalToPCUICTyping.
+
+Theorem infering_typing `{checker_flags} (Σ : global_env_ext) Γ t T (wfΣ : wf Σ) :
+  PT.wf_local Σ Γ -> Σ ;;; Γ |- t ▹ T -> Σ ;;; Γ |- t : T.
+Proof.
+  intros.
+  apply bidirectional_to_PCUIC.
+  all: assumption.
+Qed.
+
+Theorem checking_typing `{checker_flags} (Σ : global_env_ext) Γ t T (wfΣ : wf Σ) :
+  PT.wf_local Σ Γ -> PT.isType Σ Γ T -> Σ ;;; Γ |- t ◃ T -> Σ ;;; Γ |- t : T.
+Proof.
+  intros wfΓ HT Ht. revert wfΓ HT.
+  apply bidirectional_to_PCUIC.
+  all: assumption.
+Qed.
+
+Theorem infering_sort_typing `{checker_flags} (Σ : global_env_ext) Γ t u (wfΣ : wf Σ) :
+  PT.wf_local Σ Γ -> Σ ;;; Γ |- t ▸□ u -> Σ ;;; Γ |- t : tSort u.
+Proof.
+  intros wfΓ Ht. revert Ht wfΓ.
+  apply bidirectional_to_PCUIC.
+  assumption.
+Qed.
+
+Theorem infering_prod_typing `{checker_flags} (Σ : global_env_ext) Γ t na A B (wfΣ : wf Σ) :
+  PT.wf_local Σ Γ -> Σ ;;; Γ |- t ▸Π (na,A,B) -> Σ ;;; Γ |- t : tProd na A B.
+Proof.
+  intros wfΓ Ht. revert Ht wfΓ.
+  apply bidirectional_to_PCUIC.
+  assumption.
+Qed.
+
+Theorem infering_ind_typing `{checker_flags} (Σ : global_env_ext) Γ t ind u args (wfΣ : wf Σ) :
+PT.wf_local Σ Γ -> Σ ;;; Γ |- t ▸{ind} (u,args) -> Σ ;;; Γ |- t : mkApps (tInd ind u) args.
+Proof.
+  intros wfΓ Ht. revert Ht wfΓ.
+  apply bidirectional_to_PCUIC.
+  assumption.
+Qed.
+
+Theorem wf_local_bd_typing `{checker_flags} (Σ : global_env_ext) Γ (wfΣ : wf Σ) :
+  MT.wf_local Σ Γ -> PT.wf_local Σ Γ.
+Proof.
+  apply bidirectional_to_PCUIC.
+  assumption.
+Qed.
+
+Theorem wf_bd_typing `{checker_flags} (Σ : global_env_ext) (wfΣ : MT.wf Σ) :
+  PT.wf Σ.
+Proof.
+  apply bd_wf.
+  apply bidirectional_to_PCUIC.
+  assumption.
+Qed.
